SmtModuleQuery.v
@@ -43,27 +43,32 @@ Definition is_linear_chain (p : GeneralCaracaraProgram) : Prop :=
 
 (* NOTE/TODO: Open question about state equivalence and what it means for states to be equivalent for different network topologies *)
 Lemma modnet_equivalence_checker_sound :
-  forall p1 p2 f,
-  (* if two programs *)
+  forall p1 p2,
+  (* if two well-formed programs *)
   well_formed_general_program p1 ->
   well_formed_general_program p2 ->
   (* have a single source and sink *)
   is_linear_chain p1 ->
   is_linear_chain p2 ->
-  (* if they're considered equivalent *)
+  (* and they're considered equivalent *)
   modnet_equivalence_checker p1 p2 = Equivalent ->
   (* then when starting from their initial concrete states *)
-  let ci_1 := concretize_sym_modnet_state (init_general_symbolic_state "p1" p1) f in
-  let ci_2 := concretize_sym_modnet_state (init_general_symbolic_state "p2" p2) f in
-  (* they each produce a single final state *)
-  let opt_cf_1_l := eval_general_program_concrete_sinks p1 ci_1 in
-  let opt_cf_2_l := eval_general_program_concrete_sinks p2 ci_2 in
-  exists cf_1 cf_2,
-  opt_cf_1_l = Some [cf_1] /\
-  opt_cf_2_l = Some [cf_2] /\
-  (* in which the output headers are identical *)
+  forall s_i1 s_i2 c_i1 c_i2 f,
+  s_i1 = init_general_symbolic_state "p1" p1 ->
+  s_i2 = init_general_symbolic_state "p2" p2 ->
+  c_i1 = concretize_sym_modnet_state s_i1 f ->
+  c_i2 = concretize_sym_modnet_state s_i2 f ->
+  (* if they produce some final state *)
+  forall l1 l2,
+  eval_general_program_concrete_sinks p1 c_i1 = Some l1 ->
+  eval_general_program_concrete_sinks p2 c_i2 = Some l2 ->
+  (* there is only one such final state *)
+  exists c_f1 c_f2,
+  l1 = [c_f1] /\
+  l2 = [c_f2] /\
+  (* and the output headers are identical *)
   (forall h, In h (get_headers_from_general p1) ->
-    lookup_varlike cf_1 h = lookup_varlike cf_2 h).
+    lookup_varlike c_f1 h = lookup_varlike c_f2 h).
 Proof.
 Admitted.
 
@@ -78,15 +83,20 @@ Lemma modnet_equivalence_checker_complete :
   (* if they're not considered equivalent *)
   modnet_equivalence_checker p1 p2 = NotEquivalent f ->
   (* then when starting from their initial concrete states *)
-  let ci_1 := concretize_sym_modnet_state (init_general_symbolic_state "p1" p1) f in
-  let ci_2 := concretize_sym_modnet_state (init_general_symbolic_state "p2" p2) f in
+  forall s_i1 s_i2 c_i1 c_i2,
+  s_i1 = init_general_symbolic_state "p1" p1 ->
+  s_i2 = init_general_symbolic_state "p2" p2 ->
+  c_i1 = concretize_sym_modnet_state s_i1 f ->
+  c_i2 = concretize_sym_modnet_state s_i2 f ->
+  (* if they produce a some final state *)
+  forall l1 l2,
+  eval_general_program_concrete_sinks p1 c_i1 = Some l1 ->
+  eval_general_program_concrete_sinks p2 c_i2 = Some l2 ->
   (* they each produce a single final state *)
-  let opt_cf_1_l := eval_general_program_concrete_sinks p1 ci_1 in
-  let opt_cf_2_l := eval_general_program_concrete_sinks p2 ci_2 in
   exists cf_1 cf_2,
-  opt_cf_1_l = Some [cf_1] /\
-  opt_cf_2_l = Some [cf_2] /\
-  (* in which the output headers differ on at least one header *)
+  l1 = [cf_1] /\
+  l2 = [cf_2] /\
+  (* and the output headers differ on at least one header *)
   (exists h, In h (get_signature_from_general p1) /\
     lookup_varlike cf_1 h <> lookup_varlike cf_2 h).
 Proof.
